coqimp/framework/soundness/inssound.v
@@ -1,34 +1,1440 @@
 Require Import Coqlib.  
-Require Import Maps. 
+Require Import Maps.
+Require Import LibTactics.
 
 Require Import Integers.
-Open Scope Z_scope.
+Open Scope Z_scope. 
 Import ListNotations.
 
 Set Asymmetric Patterns.
-
+ 
 Require Import state. 
 Require Import language.
 
 Set Implicit Arguments.
 Unset Strict Implicit.
-
-Require Import logic.
+   
+Require Import logic. 
 Require Import soundness.
+ 
+Require Import lemmas.
+
+Require Import Coq.Logic.FunctionalExtensionality.
 
 Open Scope nat.
 Open Scope code_scope.
 
+(*+ Some Tactic +*)
+Ltac destruct_state s :=
+  destruct s as [ [ ?m [?r ?f] ] ?d ].
+
+Ltac destruct_addreq :=
+  match goal with
+  | |- context [AddrEq.eq ?x ?l] =>
+    let Heqe := fresh in
+    destruct (AddrEq.eq x l) eqn:Heqe; tryfalse; eauto
+  | _ => idtac
+  end.
+
+Ltac destruct_addreq_H :=
+  match goal with
+  | H : context [AddrEq.eq ?x ?l] |- _ =>
+    let Heqe := fresh in
+    destruct (AddrEq.eq x l) eqn:Heqe; tryfalse; eauto
+  | _ => idtac
+  end.
+
+(*+ Some Lemma +*)
+Lemma MemSet_same_addr_disj_stable :
+  forall l v v' m m',
+    disjoint (MemMap.set l (Some v') m) m' ->
+    disjoint (MemMap.set l (Some v) m) m'.
+Proof.
+  intros.
+  unfolds disjoint.
+  intros.
+  specialize (H x).
+
+  unfolds MemMap.set.
+  destruct (AddrEq.eq x l) eqn:Heqe.
+  subst.
+  destruct (m' l); tryfalse; eauto.
+
+  destruct (m x); destruct (m' x); tryfalse; eauto.
+Qed.
+
+Lemma MemSet_same_addr_disj_stable2 :
+  forall l v v' m m',
+    disjoint m (MemMap.set l (Some v') m') ->
+    disjoint m (MemMap.set l (Some v) m').
+Proof.
+  intros.
+  unfolds disjoint.
+  intro.
+  specialize (H x).
+
+  destruct (m x) eqn:Heqe1; eauto.
+  {
+    unfolds MemMap.set.
+    destruct_addreq.
+  }
+  {
+    unfolds MemMap.set.
+    destruct_addreq.
+  }
+Qed.
+  
+Lemma indom_setM_merge_eq2 :
+  forall R M rn m v,
+    ~ indom (R rn) M -> indom (R rn) m ->
+    set_R R (merge M m) rn v = merge M (set_R R m rn v).
+Proof.
+  intros.
+  eapply functional_extensionality; eauto.
+  intro.
+  unfolds set_R.
+  unfolds is_indom.
+  destruct (merge M m (R rn)) eqn:Heqe.
+  {
+    destruct (m (R rn)) eqn:Heqe1.
+    {
+      unfolds MemMap.set, merge.
+      destruct (AddrEq.eq x (R rn)) eqn:Heqe2; subst.
+      destruct (M (R rn)) eqn:Heqe3.
+      false.
+      eapply H.
+      unfold indom; eauto.
+      eauto.
+      eauto.
+    }
+    {
+      unfolds indom.
+      simpljoin1.
+      rewrite H0 in Heqe1.
+      tryfalse.
+    }
+  }
+  {
+    unfolds merge.
+    destruct (M (R rn)) eqn:Heqe1; tryfalse.
+    unfolds indom.
+    simpljoin1.
+    rewrite H0 in Heqe.
+    tryfalse.
+  }
+Qed.  
+
+Lemma disj_merge_disj_sep1 :
+  forall m1 m2 m3,
+    disjoint m1 (merge m2 m3) ->
+    disjoint m1 m2.
+Proof.
+  intros.
+  unfolds disjoint.
+  intros.
+  specialize (H x).
+  destruct (m1 x); eauto.
+  unfolds merge.
+  destruct (m2 x); eauto.
+  unfolds merge.
+  destruct (m2 x); eauto.
+Qed.
+
+Lemma disj_merge_disj_sep2 :
+  forall m1 m2 m3,
+    disjoint m1 (merge m2 m3) ->
+    disjoint m1 m3.
+Proof.
+  intros.
+  unfolds disjoint.
+  intros.
+  specialize (H x).
+  destruct (m1 x).
+  unfolds merge.
+  destruct (m2 x) eqn:Heqe1; tryfalse; eauto.
+  unfolds merge.
+  destruct (m2 x) eqn:Heqe1; tryfalse; eauto.
+  destruct (m3 x); eauto.
+Qed.
+
+Lemma memset_disj_neq :
+  forall l1 l2 v1 v2 m1 m2,
+    disjoint (MemMap.set l1 (Some v1) m1) (MemMap.set l2 (Some v2) m2) ->
+    l1 <> l2.
+Proof.
+  intros.
+  unfolds disjoint.
+  intro.
+  subst.
+  specialize (H l2).
+  unfolds MemMap.set.
+  destruct (AddrEq.eq l2 l2); tryfalse.
+Qed.
+
+Lemma memset_twice :
+  forall (A : Type) l (v v1 : A) m,
+    MemMap.set l (Some v) (MemMap.set l (Some v1) m) =
+    MemMap.set l (Some v) m.
+Proof.
+  intros.
+  eapply functional_extensionality.
+  intro.
+  unfolds MemMap.set.
+  destruct_addreq.
+Qed.
+
+Lemma memset_l_l_indom :
+  forall l v m,
+    indom l (MemMap.set l (Some v) m).
+Proof.
+  intros.
+  unfolds indom.
+  exists v.
+  unfolds MemMap.set.
+  destruct_addreq.
+Qed.
+
+Lemma disj_sep_merge_still :
+  forall m m1 m2,
+    disjoint m m1 -> disjoint m m2 ->
+    disjoint m (merge m1 m2).
+Proof.
+  intros.
+  unfolds disjoint.
+  intros.
+  specialize (H x).
+  specialize (H0 x).
+  destruct (m x) eqn:Heqe; eauto.
+  {
+    unfold merge.
+    destruct (m1 x) eqn:Heqe1; eauto.
+  }
+  {
+    unfold merge.
+    destruct (m1 x) eqn:Heqe1; eauto.
+  }
+Qed.
+
+Lemma indom_merge_still2 :
+  forall l M m,
+    indom l m ->
+    indom l (merge M m).
+Proof.
+  intros.
+  unfolds indom.
+  simpljoin1.
+  unfolds merge.
+  destruct (M l) eqn:Heqe; eauto.
+Qed.
+
+Lemma setR_merge_eq_merge_setR :
+  forall R rr v v' m1 m2,
+    set_R R (merge (MemMap.set (R rr) (Some v) m1) m2) rr v' =
+    merge (MemMap.set (R rr) (Some v') m1) m2.
+Proof.
+  intros.
+  unfolds set_R.
+  unfolds is_indom.
+  unfolds merge.
+  unfolds MemMap.set.
+  destruct_addreq.
+  eapply functional_extensionality.
+  intros.
+  destruct_addreq.
+Qed.
+
+Lemma notindom_M_setR_merge_eq :
+  forall R rn M m v,
+    ~ indom (R rn) M ->
+    set_R R (merge M m) rn v = merge M (set_R R m rn v).
+Proof.
+  intros.
+  unfolds set_R.
+  unfolds is_indom.
+  unfolds merge.
+  destruct (M (R rn)) eqn:Heqe; tryfalse.
+  {
+    eapply functional_extensionality.
+    intro.
+    unfolds MemMap.set.
+    false.
+    eapply H.
+    unfold indom.
+    eauto.
+  }
+  {
+    eapply functional_extensionality.
+    intros.
+    destruct (m (R rn)) eqn:Heqe1; eauto.
+    unfolds MemMap.set.
+    destruct_addreq; subst.
+    rewrite Heqe; eauto.
+  }
+Qed.
+
+Lemma regdlySt_set_delay_asrt_stable :
+  forall t s w M R F D rsp v,
+    regdlySt t s w (M, (R, F), D) -> ~ In rsp (getRegs D) ->
+    regdlySt t s w (M, (R, F), set_delay rsp v D).
+Proof.
+  intros t.
+  induction t; intros.
+  -
+    simpls; eauto.
+  -
+    simpls.
+    destruct H.
+    {
+      left.
+      unfolds inDlyBuff.
+      simpljoin1.
+      split.
+      {
+        unfolds set_delay.
+        simpl; eauto.
+      }
+      {
+        clear - H1 H0.
+        unfolds set_delay.
+        simpl.
+        econstructor; eauto.
+      }
+    }
+    {
+      right.
+      eauto.
+    }
+Qed.
+
+Lemma notin_dom_set_delay_asrt_stable :
+  forall p M R F D (rsp : SpReg) v,
+    (M, (R, F), D) |= p ->
+    ~ indom (R rsp) M -> ~ In rsp (getRegs D) ->
+    (M, (R, F), set_delay rsp v D) |= p.
+Proof.
+  intro p.
+  induction p; intros; simpls; eauto.
+
+  -
+    unfolds regSt.
+    simpls.
+    simpljoin1.
+    repeat (split; eauto).
+
+    assert ((R rsp) <> (R r)).
+    {
+      clear - H0.
+      intro.
+      eapply H0.
+      unfold indom.
+      rewrite H.
+      eexists.
+      unfolds MemMap.set.
+      destruct_addreq.
+    }
+ 
+    intro.
+    clear - H H3 H2.
+    unfolds regInDlyBuff.
+    destruct r; tryfalse.
+    unfolds set_delay. 
+    simpl in H3.
+    destruct H3; subst. 
+    eapply H; eauto.
+    tryfalse.
+
+  - 
+    simpljoin1.
+    exists x.
+    repeat (split; eauto).
+    destruct H2.
+    { 
+      left.
+      eapply regdlySt_set_delay_asrt_stable; eauto.
+    }
+    {
+      right.
+      unfolds regSt.
+      simpls.
+      simpljoin1.
+      repeat (split; eauto).
+      intro.
+      destruct H3.
+      {
+        subst.
+        eapply H0.
+        unfold indom.
+        exists x.
+        unfold MemMap.set.
+        destruct_addreq.
+      }
+      {
+        tryfalse.
+      }
+    }
+
+  -
+    simpljoin1.
+    eapply IHp1 in H; eauto.
+
+  -
+    destruct H.
+    eapply IHp1 in H; eauto.
+    eapply IHp2 in H; eauto.
+
+  -
+    simpljoin1.
+    destruct_state x.
+    destruct_state x0.
+    simpl in H.
+    simpljoin1.
+    exists (m, (r0, f0), set_delay rsp v d0) (m0, (r0, f0), set_delay rsp v d0).
+    simpl.
+    repeat (split; eauto).
+    eapply IHp1; eauto.
+    clear - H0.
+    intro.
+    eapply H0.
+    eapply indom_merge_still; eauto.
+    eapply IHp2; eauto.
+    clear - H0.
+    intro.
+    eapply H0.
+    eapply indom_merge_still2; eauto.
+
+  -
+    simpljoin1.
+    exists x.
+    eauto.
+Qed.
+    
 (*+ Soundness Proof of instruction +*)
-Theorem ins_rule_sound : forall p q i,
-    |- {{ p }} i {{ q }} ->
-    ins_sound p q i.
+
+Lemma ld_rule_sound :
+  forall p q aexp l v v' (rd : GenReg),
+    p ==> aexp ==ₓ l ->
+    p ==> l |-> v ** rd |=> v' ** q ->
+    ins_sound p (l |-> v ** rd |=> v ** q) (ld aexp rd).
+Proof.
+  intros.
+  unfolds ins_sound.
+  intros.
+  lets Ht : H1.
+  eapply H in H1.
+  eapply H0 in Ht.
+  simpl in Ht.
+  simpljoin1.
+  destruct_state s.
+  destruct_state x.
+  destruct_state x0.
+  destruct_state x1.
+  destruct_state x2.
+  simpl in H2.
+  simpljoin1.
+  simpl in H3.
+  simpl in H4.
+  simpljoin1.
+  eexists.
+  split.
+ 
+  Focus 2.
+  simpl.
+  do 2 eexists.
+  repeat split.
+  Focus 2.
+  instantiate (1 := (MemMap.set l (Some v) emp, (r3, f3), d3)).
+  simpl; eauto.
+
+  Focus 2.
+  exists (MemMap.set (r3 rd) (Some v) emp, (r3, f3), d3) (m3, (r3, f3), d3).
+  split.
+  simpl.
+  repeat (split; eauto).
+
+  clear - H4 H5.
+  unfolds regSt.
+  simpljoin1.
+  simpls.
+  subst.
+  eapply MemSet_same_addr_disj_stable; eauto.
+
+  split; eauto.
+  clear - H5.
+  unfolds regSt.
+  simpljoin1.
+  simpls.
+  subst.
+  split; eauto.
+
+  simpl.
+  repeat (split; eauto).
+  
+  clear - H5 H4 H2.
+  unfolds regSt.
+  simpljoin1.
+  simpls.
+  subst.
+  clear - H2.
+  unfolds disjoint.
+  intro.
+  specialize (H2 x).
+  destruct (MemMap.set l (Some v) emp x) eqn:Heqe.
+  unfolds merge.
+  clear - H2.
+  unfolds MemMap.set.
+  destruct (AddrEq.eq x (r3 rd)); tryfalse; eauto.
+  unfolds merge.
+  clear - H2.
+  unfolds MemMap.set.
+  destruct (AddrEq.eq x (r3 rd)); tryfalse; eauto.
+
+  econstructor.
+  econstructor; eauto.
+
+  instantiate (1 := l).
+  clear - H1.
+  simpl in H1.
+  destruct H1; eauto.
+  simpl in H1.
+  destruct H1; eauto.
+ 
+  instantiate (1 := v).
+  unfold merge, MemMap.set.
+  destruct (AddrEq.eq l l); tryfalse; eauto.
+  
+  clear - H5 H2 H4.
+  unfolds regSt.
+  simpljoin1.
+  simpls; subst. 
+  unfold indom.
+  exists v'.
+  unfold merge.
+  eapply disj_merge_disj_sep1 in H2.
+  clear - H2.
+  eapply memset_disj_neq in H2.
+  unfolds MemMap.set.
+  destruct (AddrEq.eq (r3 rd) l); tryfalse.
+  simpl. 
+  destruct (AddrEq.eq (r3 rd) (r3 rd)); eauto; tryfalse.
+  erewrite indom_setM_merge_eq2; eauto.
+  unfolds regSt.
+  simpljoin1.
+  simpls; subst.
+  clear.
+  rewrite indom_setR_merge_eq; eauto.
+  unfold set_R.
+ 
+  assert (is_indom (r3 rd) (MemMap.set (r3 rd) (Some v') emp) = true).
+  {
+    unfolds is_indom, MemMap.set.
+    destruct (AddrEq.eq (r3 rd) (r3 rd)); tryfalse.
+    eauto.
+  }
+  rewrite H; eauto.
+  rewrite memset_twice; eauto.
+
+  unfold indom.
+  eexists.
+  unfolds MemMap.set.
+  destruct_addreq.
+
+  intro.
+  eapply disj_merge_disj_sep1 in H2.
+  unfolds regSt.
+  simpls; simpljoin1; eauto.
+  eapply memset_disj_neq in H2.
+  clear - H2 H3.
+  unfolds indom.
+  simpljoin1.
+  unfolds MemMap.set.
+  destruct_addreq_H.
+
+  clear - H5.
+  unfolds regSt.
+  simpljoin1.
+  simpls.
+  subst.
+  unfold indom.
+  exists v'.
+  unfold merge, MemMap.set.
+  destruct_addreq.
+Qed.
+
+Lemma st_rule_sound :
+  forall l v (rs : GenReg) v1 p aexp,
+    l |-> v ** rs |=> v1 ** p ==> aexp ==ₓ l ->
+    ins_sound (l |-> v ** rs |=> v1 ** p) (l |-> v1 ** rs |=> v1 ** p) (st rs aexp).
 Proof.
   intros.
   unfold ins_sound.
-  destruct i; intros.
-  - (* ld aexp rd *)
-    rename a into aexp; rename g into rd.
-    inversion H1; subst.
-    inversion H; subst.
+  intros.
+  lets Ht : H0.
+  simpl in H0.
+  simpljoin1.
+  destruct_state s.
+  destruct_state x.
+  destruct_state x0.
+  destruct_state x1.
+  destruct_state x2.
+
+  simpl in H2.
+  simpljoin1.
+  simpl in H0, H1.
+  simpljoin1.
+  unfolds regSt.
+  simpl in H3.
+  simpljoin1.
+
+  eexists.
+  split.
+
+  Focus 2.
+  simpl. 
+  exists (MemMap.set l (Some v1) emp, (r3, f3), d3). eexists.
+   
+  repeat split.
+
+  Focus 2.
+  exists (MemMap.set (r3 rs) (Some v1) emp, (r3, f3), d3) (m3, (r3, f3), d3).
+  repeat (split; eauto).
+
+  simpl.
+  repeat (split; eauto).
+  eapply MemSet_same_addr_disj_stable; eauto.
+
+  do 2 econstructor; eauto.
+  eapply H in Ht.
+  simpl in Ht.
+  simpljoin1; eauto.
+  eapply H in Ht.
+  simpl in Ht.
+  simpljoin1; eauto.
+
+  eapply disj_merge_disj_sep1 in H0.
+  eapply memset_disj_neq in H0.
+  instantiate (1 := v1).
+  clear - H0.
+  unfold merge, MemMap.set.
+  destruct_addreq.
+  simpl.
+  destruct_addreq.
+  eapply indom_merge_still; eauto.
+  eapply memset_l_l_indom; eauto.
+
+  rewrite indom_setM_merge_eq; eauto.
+  rewrite memset_twice; eauto.
+  eapply memset_l_l_indom; eauto.
+Qed.
+
+Lemma add_rule_sound :
+  forall p (rs rd : GenReg) v1 v2 v oexp q,
+    p ==> Or rs ==ₑ v1 //\\ oexp ==ₑ v2 ->
+    p ==> rd |=> v ** q ->
+    ins_sound p (rd |=> v1 +ᵢ v2 ** q) (add rs oexp rd).
+Proof.
+  intros.
+  unfolds ins_sound.
+  intros.
+  lets Ht : H1.
+  eapply H in H1.
+  eapply H0 in Ht.
+
+  simpl in Ht.
+  simpljoin1.
+  destruct_state s.
+  destruct_state x.
+  destruct_state x0.
+
+  simpl in H2.
+  simpljoin1.
+  unfolds regSt.
+  simpl in H3.
+  simpljoin1.
+
+  simpl in H1.
+  simpljoin1.
+
+  eexists.
+  split.
+
+  Focus 2.
+  simpl.
+  do 2 eexists.
+
+  split.
+  Focus 2.
+  split.
+  instantiate (1 := (MemMap.set (r1 rd) (Some v1 +ᵢ v2) emp, (r1, f1), d1)).
+  unfold regSt.
+  simpl.
+  split; eauto.
+  eauto.
+
+  simpl.
+  repeat (split; eauto).
+  eapply MemSet_same_addr_disj_stable; eauto.
+
+  do 2 econstructor; eauto.
+  eapply indom_merge_still; eauto.
+  eapply memset_l_l_indom; eauto.
+
+  rewrite indom_setM_merge_eq; eauto.
+  rewrite memset_twice; eauto.
+  eapply memset_l_l_indom; eauto.
+Qed.
+
+Lemma sub_rule_sound :
+  forall p (rs rd : GenReg) v1 v2 v oexp q,
+    p ==> Or rs ==ₑ v1 //\\ oexp ==ₑ v2 ->
+    p ==> rd |=> v ** q ->
+    ins_sound p (rd |=> v1 -ᵢ v2 ** q) (sub rs oexp rd).
+Proof.
+  intros.
+  unfolds ins_sound.
+  intros.
+  lets Ht : H1.
+  eapply H in H1.
+  eapply H0 in Ht.
+
+  simpl in Ht.
+  simpljoin1.
+  destruct_state s.
+  destruct_state x.
+  destruct_state x0.
+
+  simpl in H2.
+  simpljoin1.
+  unfolds regSt.
+  simpl in H3.
+  simpljoin1.
+
+  simpl in H1.
+  simpljoin1.
+
+  eexists.
+  split.
+
+  Focus 2.
+  simpl.
+  do 2 eexists.
+
+  split.
+  Focus 2.
+  split.
+  instantiate (1 := (MemMap.set (r1 rd) (Some v1 -ᵢ v2) emp, (r1, f1), d1)).
+  unfold regSt.
+  simpl.
+  split; eauto.
+  eauto.
+
+  simpl.
+  repeat (split; eauto).
+  eapply MemSet_same_addr_disj_stable; eauto.
+
+  do 2 econstructor; eauto.
+  eapply indom_merge_still; eauto.
+  eapply memset_l_l_indom; eauto.
+
+  rewrite indom_setM_merge_eq; eauto.
+  rewrite memset_twice; eauto.
+  eapply memset_l_l_indom; eauto.
+Qed.
+
+Lemma subcc_rule_sound :
+  forall p oexp (r1 r2 : GenReg) v1 v2 v vr vn vz q,
+    p ==> Or r1 ==ₑ v1 //\\ oexp ==ₑ v2 -> v = v1 -ᵢ v2 ->
+    p ==> r2 |=> vr ** n |=> vn ** z |=> vz ** q ->
+    ins_sound p (r2 |=> v ** n |=> get_range 31 31 v ** z |=> iszero v ** q)
+              (subcc r1 oexp r2).
+Proof.
+  intros.
+  unfold ins_sound.
+  intros.
+  lets Ht : H2.
+  eapply H in H2.
+  eapply H1 in Ht.
+
+  simpl in Ht.
+  simpljoin1.
+  destruct_state s.
+  destruct_state x0.
+  destruct_state x.
+  destruct_state x1.
+  destruct_state x2.
+  destruct_state x3.
+  destruct_state x4.
+
+  unfolds regSt.
+  simpljoin1.
+  simpl in H3, H4, H5, H6, H7, H0.
+  simpljoin1.
+
+  eexists.
+  split.
+  
+  Focus 2.
+  simpl.  
+  exists (MemMap.set (r7 r2) (Some v1 -ᵢ v2) emp, (r7, f5), d5).    
+  eexists.
+  split. 
+  Focus 2.
+  split. 
+  unfold regSt.
+  simpl; eauto.
+
+  exists (MemMap.set (r7 n) (Some (get_range 31 31 v1 -ᵢ v2)) emp, (r7, f5), d5).
+  eexists.
+  
+  split.
+  Focus 2.
+  split.
+  unfold regSt.
+  simpl; eauto.
+
+  exists (MemMap.set (r7 z) (Some (iszero v1 -ᵢ v2)) emp, (r7, f5), d5).
+  eexists.
+
+  split.
+  Focus 2.
+  split.
+  unfold regSt.
+  simpl; eauto.
+  eauto.
+ 
+  simpl.
+  repeat (split; eauto).
+  eapply MemSet_same_addr_disj_stable; eauto.
+
+  simpl.
+  repeat (split; eauto).
+  eapply disj_sep_merge_still; eauto.
+ 
+  clear - H5.
+  eapply disj_merge_disj_sep1 in H5.
+  eapply MemSet_same_addr_disj_stable.
+  eapply MemSet_same_addr_disj_stable2; eauto.  
+
+  clear - H5.
+  eapply disj_merge_disj_sep2 in H5.
+  eapply MemSet_same_addr_disj_stable; eauto.
+
+  simpl.
+  repeat (split; eauto).
+
+  clear - H3.
+  eapply disj_sep_merge_still.
+
+  eapply disj_merge_disj_sep1 in H3.
+  eapply MemSet_same_addr_disj_stable2; eauto.
+  eapply MemSet_same_addr_disj_stable; eauto.
+
+  eapply disj_sep_merge_still.
+  eapply disj_merge_disj_sep2 in H3.
+  eapply disj_merge_disj_sep1 in H3.
+  eapply MemSet_same_addr_disj_stable.
+  eapply MemSet_same_addr_disj_stable2; eauto.
+
+  eapply disj_merge_disj_sep2 in H3.
+  eapply disj_merge_disj_sep2 in H3.
+  eapply MemSet_same_addr_disj_stable; eauto.
+
+  do 2 econstructor; eauto.
+  {
+    instantiate (1 := v1).
+    clear - H2.
+    simpl in H2.
+    simpljoin1.
+    clear - H.
+    unfolds eval_reg.
+    eauto.
+  }
+  {
+    instantiate (1 := v2).
+    clear - H2.
+    simpl in H2.
+    simpljoin1; eauto.
+  }
+  {
+    eapply indom_merge_still.
+    eapply memset_l_l_indom; eauto.
+  }
+  {
+    eapply indom_merge_still2; eauto.
+    eapply indom_merge_still.
+    eapply memset_l_l_indom; eauto.
+  }
+  {
+    do 2 eapply indom_merge_still2.
+    eapply indom_merge_still.
+    eapply memset_l_l_indom; eauto.
+  } 
+  {
+    unfolds set_Rs.
+    rewrite setR_merge_eq_merge_setR.
+    rewrite notindom_M_setR_merge_eq; eauto.
+    rewrite notindom_M_setR_merge_eq; eauto.
+    rewrite setR_merge_eq_merge_setR.
+    rewrite notindom_M_setR_merge_eq; eauto.
+    rewrite setR_merge_eq_merge_setR.
+    eauto.
+
+    clear - H5.
+    eapply disj_merge_disj_sep1 in H5.
+    eapply memset_disj_neq in H5.
+    intro.
+    unfolds indom.
+    simpljoin1.
+    unfolds MemMap.set.
+    destruct_addreq_H.
+
+    clear - H3.
+    eapply disj_merge_disj_sep2 in H3.
+    eapply disj_merge_disj_sep1 in H3.
+    eapply memset_disj_neq in H3.
+    intro.
+    unfolds indom.
+    simpljoin1.
+    unfolds MemMap.set.
+    destruct_addreq_H.
+
+    clear - H3.
+    eapply disj_merge_disj_sep1 in H3.
+    eapply memset_disj_neq in H3.
+    intro.
+    unfolds indom.
+    simpljoin1.
+    unfolds MemMap.set.
+    destruct_addreq_H.
+  }
+Qed.
+
+Lemma and_rule_sound :
+  forall p (rs rd : GenReg) v1 v2 v oexp q,
+    p ==> Or rs ==ₑ v1 //\\ oexp ==ₑ v2 ->
+    p ==> rd |=> v ** q ->
+    ins_sound p (rd |=> v1 &ᵢ v2 ** q) (and rs oexp rd).
+Proof.
+  intros.
+  unfolds ins_sound.
+  intros.
+  lets Ht : H1.
+  eapply H in H1.
+  eapply H0 in Ht.
+
+  simpl in Ht.
+  simpljoin1.
+  destruct_state s.
+  destruct_state x.
+  destruct_state x0.
+
+  simpl in H2.
+  simpljoin1.
+  unfolds regSt.
+  simpl in H3.
+  simpljoin1.
+
+  simpl in H1.
+  simpljoin1.
+
+  eexists.
+  split.
+
+  Focus 2.
+  simpl.
+  do 2 eexists.
+
+  split.
+  Focus 2.
+  split.
+  instantiate (1 := (MemMap.set (r1 rd) (Some v1 &ᵢ v2) emp, (r1, f1), d1)).
+  unfold regSt.
+  simpl.
+  split; eauto.
+  eauto.
+
+  simpl.
+  repeat (split; eauto).
+  eapply MemSet_same_addr_disj_stable; eauto.
+ 
+  do 2 econstructor; eauto. 
+  eapply indom_merge_still; eauto.
+  eapply memset_l_l_indom; eauto.
+ 
+  rewrite indom_setM_merge_eq; eauto.
+  rewrite memset_twice; eauto.
+  eapply memset_l_l_indom; eauto.
+Qed.
+
+Lemma andcc_rule_sound :
+  forall p oexp (r1 r2 : GenReg) v1 v2 v vr vn vz q,
+    p ==> Or r1 ==ₑ v1 //\\ oexp ==ₑ v2 -> v = v1 &ᵢ v2 ->
+    p ==> r2 |=> vr ** n |=> vn ** z |=> vz ** q ->
+    ins_sound p (r2 |=> v ** n |=> get_range 31 31 v ** z |=> iszero v ** q)
+              (andcc r1 oexp r2).
+Proof.
+  intros.
+  unfold ins_sound.
+  intros.
+  lets Ht : H2.
+  eapply H in H2.
+  eapply H1 in Ht.
+
+  simpl in Ht.
+  simpljoin1.
+  destruct_state s.
+  destruct_state x0.
+  destruct_state x.
+  destruct_state x1.
+  destruct_state x2.
+  destruct_state x3.
+  destruct_state x4.
+
+  unfolds regSt.
+  simpljoin1.
+  simpl in H3, H4, H5, H6, H7, H0.
+  simpljoin1.
+
+  eexists.
+  split.
+  
+  Focus 2.
+  simpl.  
+  exists (MemMap.set (r7 r2) (Some v1 &ᵢ v2) emp, (r7, f5), d5).    
+  eexists.
+  split. 
+  Focus 2. 
+  split. 
+  unfold regSt.
+  simpl; eauto.
+
+  exists (MemMap.set (r7 n) (Some (get_range 31 31 v1 &ᵢ v2)) emp, (r7, f5), d5).
+  eexists.
+  
+  split.
+  Focus 2.
+  split.
+  unfold regSt.
+  simpl; eauto.
+
+  exists (MemMap.set (r7 z) (Some (iszero v1 &ᵢ v2)) emp, (r7, f5), d5).
+  eexists.
+
+  split.
+  Focus 2.
+  split.
+  unfold regSt.
+  simpl; eauto.
+  eauto.
+ 
+  simpl.
+  repeat (split; eauto).
+  eapply MemSet_same_addr_disj_stable; eauto.
+
+  simpl.
+  repeat (split; eauto).
+  eapply disj_sep_merge_still; eauto.
+ 
+  clear - H5.
+  eapply disj_merge_disj_sep1 in H5.
+  eapply MemSet_same_addr_disj_stable.
+  eapply MemSet_same_addr_disj_stable2; eauto.  
+
+  clear - H5.
+  eapply disj_merge_disj_sep2 in H5.
+  eapply MemSet_same_addr_disj_stable; eauto.
+
+  simpl.
+  repeat (split; eauto).
+
+  clear - H3.
+  eapply disj_sep_merge_still.
+
+  eapply disj_merge_disj_sep1 in H3.
+  eapply MemSet_same_addr_disj_stable2; eauto.
+  eapply MemSet_same_addr_disj_stable; eauto.
+
+  eapply disj_sep_merge_still.
+  eapply disj_merge_disj_sep2 in H3.
+  eapply disj_merge_disj_sep1 in H3.
+  eapply MemSet_same_addr_disj_stable.
+  eapply MemSet_same_addr_disj_stable2; eauto.
+
+  eapply disj_merge_disj_sep2 in H3.
+  eapply disj_merge_disj_sep2 in H3.
+  eapply MemSet_same_addr_disj_stable; eauto.
+
+  do 2 econstructor; eauto.
+  {
+    instantiate (1 := v1).
+    clear - H2.
+    simpl in H2.
+    simpljoin1.
+    clear - H.
+    unfolds eval_reg.
+    eauto.
+  }
+  {
+    instantiate (1 := v2).
+    clear - H2.
+    simpl in H2.
+    simpljoin1; eauto.
+  }
+  {
+    eapply indom_merge_still.
+    eapply memset_l_l_indom; eauto.
+  }
+  {
+    eapply indom_merge_still2; eauto.
+    eapply indom_merge_still.
+    eapply memset_l_l_indom; eauto.
+  }
+  {
+    do 2 eapply indom_merge_still2.
+    eapply indom_merge_still.
+    eapply memset_l_l_indom; eauto.
+  } 
+  {
+    unfolds set_Rs.
+    rewrite setR_merge_eq_merge_setR.
+    rewrite notindom_M_setR_merge_eq; eauto.
+    rewrite notindom_M_setR_merge_eq; eauto.
+    rewrite setR_merge_eq_merge_setR.
+    rewrite notindom_M_setR_merge_eq; eauto.
+    rewrite setR_merge_eq_merge_setR.
+    eauto.
+
+    clear - H5.
+    eapply disj_merge_disj_sep1 in H5.
+    eapply memset_disj_neq in H5.
+    intro.
+    unfolds indom.
+    simpljoin1.
+    unfolds MemMap.set.
+    destruct_addreq_H.
+
+    clear - H3.
+    eapply disj_merge_disj_sep2 in H3.
+    eapply disj_merge_disj_sep1 in H3.
+    eapply memset_disj_neq in H3.
+    intro.
+    unfolds indom.
+    simpljoin1.
+    unfolds MemMap.set.
+    destruct_addreq_H.
+
+    clear - H3.
+    eapply disj_merge_disj_sep1 in H3.
+    eapply memset_disj_neq in H3.
+    intro.
+    unfolds indom.
+    simpljoin1.
+    unfolds MemMap.set.
+    destruct_addreq_H.
+  }
+Qed.
+
+Lemma or_rule_sound :
+  forall p (rs rd : GenReg) v1 v2 v oexp q,
+    p ==> Or rs ==ₑ v1 //\\ oexp ==ₑ v2 ->
+    p ==> rd |=> v ** q ->
+    ins_sound p (rd |=> v1 |ᵢ v2 ** q) (or rs oexp rd).
+Proof.
+  intros.
+  unfolds ins_sound.
+  intros.
+  lets Ht : H1.
+  eapply H in H1.
+  eapply H0 in Ht.
+
+  simpl in Ht.
+  simpljoin1.
+  destruct_state s.
+  destruct_state x.
+  destruct_state x0.
+
+  simpl in H2.
+  simpljoin1.
+  unfolds regSt.
+  simpl in H3.
+  simpljoin1.
+
+  simpl in H1.
+  simpljoin1.
+
+  eexists.
+  split.
+
+  Focus 2.
+  simpl.
+  do 2 eexists.
+
+  split.
+  Focus 2.
+  split.
+  instantiate (1 := (MemMap.set (r1 rd) (Some v1 |ᵢ v2) emp, (r1, f1), d1)).
+  unfold regSt.
+  simpl.
+  split; eauto.
+  eauto.
+
+  simpl.
+  repeat (split; eauto).
+  eapply MemSet_same_addr_disj_stable; eauto.
+ 
+  do 2 econstructor; eauto. 
+  eapply indom_merge_still; eauto.
+  eapply memset_l_l_indom; eauto.
+ 
+  rewrite indom_setM_merge_eq; eauto.
+  rewrite memset_twice; eauto.
+  eapply memset_l_l_indom; eauto.
+Qed.
+
+Lemma nop_rule_sound :
+  forall p q,
+    p ==> q -> ins_sound p q nop.
+Proof.
+  intros.
+  unfolds ins_sound.
+  intros.
+  exists s.
+  split; eauto.
+  destruct_state s.
+  do 2 econstructor.
+Qed.
+
+Lemma rd_rule_sound :
+  forall (rsp : SpReg) (r1 : GenReg) v v1 p,
+    ins_sound (rsp |=> v ** r1 |=> v1 ** p) (rsp |=> v ** r1 |=> v ** p) (rd rsp r1).
+Proof.
+  intros.
+  unfolds ins_sound.
+  intros.
+  destruct_state s.
+  simpl in H.
+  simpljoin1.
+  destruct_state x0.
+  destruct_state x.
+  destruct_state x1.
+  destruct_state x2.
+
+  simpl in H.
+  simpljoin1.
+  simpl in H1.
+  simpljoin1.
+
+  unfolds regSt.
+  simpls.
+  simpljoin1.
+
+  eexists.
+  split.
+  Focus 2.
+  exists (MemMap.set (r4 rsp) (Some v) emp, (r4, f3), d3).
+  eexists.
+
+  split.
+  Focus 2.
+  split.
+  unfold regSt; simpl.
+  split; eauto.
+
+  exists (MemMap.set (r4 r1) (Some v) emp, (r4, f3), d3). eexists.
+  split.
+  Focus 2.
+  unfold regSt.
+  simpls; eauto.
+  repeat (split; eauto). 
+  eapply MemSet_same_addr_disj_stable; eauto.
+
+  simpl.
+  repeat (split; simpl; eauto).
+  eapply disj_sep_merge_still.
+  eapply disj_merge_disj_sep1 in H. 
+  eapply MemSet_same_addr_disj_stable2; eauto.
+  eapply disj_merge_disj_sep2 in H.
+  eapply MemSet_same_addr_disj_stable; eauto.
+
+  do 2 econstructor.
+  instantiate (1 := v).
+  unfold merge, MemMap.set.
+  destruct_addreq.
+  eapply indom_merge_still2.
+  eapply indom_merge_still.
+  eapply memset_l_l_indom; eauto.
+
+  rewrite indom_setM_merge_eq2; eauto.
+  rewrite setR_merge_eq_merge_setR; eauto.
+
+  intro.
+  eapply disj_merge_disj_sep1 in H.
+  eapply memset_disj_neq in H; eauto.
+  clear - H0 H.
+  unfolds indom.
+  simpljoin1.
+  unfolds MemMap.set.
+  destruct_addreq_H.
+
+  eapply indom_merge_still.
+  eapply memset_l_l_indom; eauto.
+Qed.
+
+Lemma wr_rule_sound :
+  forall (rsp : SpReg) v p (rs : GenReg) oexp v1 v2,
+    rsp |=> v ** p ==> Or rs ==ₑ v1 //\\ oexp ==ₑ v2 ->
+    ins_sound (rsp |=> v ** p) (3 @ rsp |==> v1 xor v2 ** p) (wr rs oexp rsp).
+Proof.
+  intros.
+  unfolds ins_sound.
+  intros.
+  destruct_state s.
+  lets Ht : H0.
+  eapply H in H0.
+  simpl in Ht.
+  simpljoin1.
+  destruct_state x.
+  destruct_state x0.
+
+  simpl in H1.
+  simpljoin1.
+  unfolds regSt.
+  simpl in H2.
+  simpljoin1.
+  eexists.
+ 
+  split.
+  Focus 2.  
+  exists (MemMap.set (r1 rsp) (Some v) emp, (r1, f1), set_delay rsp v1 xor v2 d1).
+  eexists.
+
+  split.
+  Focus 2.
+  instantiate (1 := (m1, (r1, f1), set_delay rsp v1 xor v2 d1)).
+  split; eauto.
+  simpl.
+  exists v.
+  repeat (split; eauto).
+  eapply notin_dom_set_delay_asrt_stable; eauto.
+  clear - H1.
+  intro.
+  unfolds indom.
+  simpljoin1.
+  unfolds disjoint.
+  specialize (H1 (r1 rsp)).
+  unfolds MemMap.set.
+  destruct_addreq_H.
+  rewrite H in H1.
+  tryfalse.
+  
+  simpl.
+  repeat (split; eauto).
+
+  eapply Wr.
+  instantiate (1 := v1).
+  clear - H0.
+  simpl in H0.
+  simpljoin1; eauto.
+  simpl in H0.
+  simpljoin1; eauto.
+  eauto.
+
+  eapply indom_merge_still; eauto.
+  eapply memset_l_l_indom; eauto.
+  eauto.
+Qed.
+
+Lemma sep_star_split :
+  forall s p1 p2,
+    s |= p1 ** p2 ->
+    exists s1 s2, s1 |= p1 /\ s2 |= p2 /\ state_union s1 s2 s.
+Proof.
+  intros.
+  simpl in H.
+  simpljoin1; eauto.
+Qed.
+  
+Lemma save_rule_sound :
+  forall p q (rs rd : GenReg) v1 v2 v v' id id' F fm1 fm2 fmo fml fmi p1 oexp,
+    p ==> Or rs ==ₑ v1 //\\ oexp ==ₑ v2 ->
+    p ==> {|id, F ++ [fm1; fm2]|} ** Regs fmo fml fmi ** p1 ->
+    id' = pre_cwp id -> win_masked id' v = false ->
+    {|id', fml :: fmi :: F|} ** Regs fm1 fm2 fmo ** p1 ==> rd |=> v' ** q ->
+    ins_sound (Rwim |=> v ** p) (Rwim |=> v ** rd |=> v1 +ᵢ v2 ** q) (save rs oexp rd).
+Proof.
+  intros.
+  unfolds ins_sound.
+  intros.
+  destruct_state s.
+  simpl in H4.
+  simpljoin1.
+  destruct_state x.
+  destruct_state x0.
+  simpl in H4.
+  simpljoin1.
+
+  lets Ht : H6.
+  lets Ht1 : H6.
+  eapply H0 in H6.
+
+  eapply sep_star_split in H6.
+  simpljoin1.
+  destruct_state x.
+  destruct_state x0.
+
+  simpl in H7.
+  simpljoin1.
+  eapply sep_star_split in H6; eauto.
+  simpljoin1.
+  destruct_state x.
+  destruct_state x0.
+  simpl in H9.
+  simpljoin1.
+
+  eexists.
+  split.
+  {
+    
+  }
+  
+Theorem ins_rule_sound : forall p q i,
+      |- {{ p }} i {{ q }} ->
+      ins_sound p q i.
+Proof.
+  intros.
+  induction H. 
+ 
+  - (* ld *)
+    eapply ld_rule_sound; eauto.
+
+  - (* st *)
+    eapply st_rule_sound; eauto.
+
+  - (* add *)
+    eapply add_rule_sound; eauto.
+
+  - (* sub *)
+    eapply sub_rule_sound; eauto.
+
+  - (* subcc *) 
+    eapply subcc_rule_sound; eauto.
+
+  - (* and *)
+    eapply and_rule_sound; eauto.
+
+  - (* andcc *)
+    eapply andcc_rule_sound; eauto.
+
+  - (* or *)
+    eapply or_rule_sound; eauto.
+
+  - (* nop *)
+    eapply nop_rule_sound; eauto.
+
+  - (* rd *)
+    eapply rd_rule_sound; eauto.
+ 
+  - (* wr *)
+    eapply wr_rule_sound; eauto.
+
+  - (* save *)
     
