coqimp/framework/soundness/sep_tactic.v
@@ -1,0 +1,117 @@
+Require Import Coqlib.  
+Require Import Maps.
+Require Import LibTactics.
+
+Require Import Integers.
+Open Scope Z_scope. 
+Import ListNotations.
+
+Set Asymmetric Patterns.
+ 
+Require Import state. 
+Require Import language.
+
+Set Implicit Arguments.
+Unset Strict Implicit.
+ 
+Require Import logic.
+Require Import soundness.
+ 
+Require Import lemmas.
+
+Open Scope nat.
+Open Scope code_scope.
+
+(*+ Some tactic for Sep Proof +*)
+Fixpoint asrt_to_lst (a : asrt) : list asrt :=
+  match a with
+  | p ** q => p :: asrt_to_lst q
+  | _ => a :: nil
+  end.
+
+Fixpoint lst_to_asrt (ls : list asrt) : asrt :=
+  match ls with
+  | a :: nil => a
+  | a :: ls' => a ** lst_to_asrt ls'
+  | nil => Aemp
+  end.
+
+Fixpoint lift_n' {A : Type} (ls : list A) (n : nat) (prels : list A) :=
+  match n with
+  | S n' =>
+    match ls with
+    | a :: ls' => lift_n' ls' n' (prels ++ (a :: nil))
+    | nil => prels ++ ls
+    end
+  | O =>
+    match ls with
+    | a :: ls' => a :: prels ++ ls'
+    | nil => prels
+    end
+  end.
+
+Definition lift_n {A : Type} (ls : list A) (n : nat) :=
+  lift_n' ls n nil.
+
+Lemma asrt_to_lst_nil_false :
+  forall p,
+    asrt_to_lst p = nil -> False.
+Proof.
+  intro p.
+  induction p; intros;
+    simpls; tryfalse.
+Qed.
+  
+Lemma sep_lift_stable :
+  forall p s ls n,
+    s |= p -> asrt_to_lst p = ls ->
+    s |= lst_to_asrt (lift_n ls n).
+Proof.
+  intro p.
+  induction p; intros;
+    try solve
+      [
+        simpls; subst; destruct n; simpl; eauto;
+        unfold lift_n; simpl; destruct n; eauto
+      ].
+
+  -
+    subst.
+    destruct n0; simpl; eauto.
+    unfold lift_n.
+    simpl.
+    destruct n0; eauto.
+
+  -
+    simpl in H0.
+    destruct ls; tryfalse.
+    inversion H0.
+    subst.
+    clear H0.
+    simpl in H.
+    simpljoin1.
+    renames x to s1, x0 to s2.
+    unfold lift_n.  
+    simpl lift_n'.
+    destruct n.
+    { 
+      simpl lst_to_asrt.
+      destruct (asrt_to_lst p2) eqn:Heqe.
+      {
+        eapply asrt_to_lst_nil_false in Heqe; tryfalse.
+      }
+      {
+        simpl sat.
+        exists s1 s2.
+        repeat (split; eauto).
+        destruct l.
+        eapply IHp2 with (ls := [a0]) (n := 0) in H1; eauto.
+        eapply IHp2 with (ls := a0 :: a1 :: l) (n := 0) in H1; eauto.
+      }
+    }
+    {
+      
+    }
+  
+
+
